too difficult

Others/Aha.v
@@ -1,36 +1,66 @@
-Require Import List.
-Require Import Nat.
-
-Import ListNotations.
+Require Import Init.Datatypes.
+From Coq Require Recdef.
+Require Import Init.Nat.
+From Coq Require Import Lia.
 
 Inductive Term :=
-| true
-| false
+| t
+| f
 | zero
 | succ (t : Term)
 | pred (t : Term)
 | iszero (t : Term)
-| cond : Term -> Term -> Term -> Term.
+| cond (p : Term) (t1 : Term) (t2 : Term).
 
-Compute (succ (succ zero)).
-
-Fixpoint eval (t: Term) : Term :=
+Fixpoint isnv (t: Term) : bool :=
     match t with
-    | succ t' => succ (eval t')
-    | iszero zero => true
-    (* FIX LATER *)
-    | iszero (succ _) => false
-    | pred t' => match eval t' with
-        | zero => zero
-        | succ t'' => t''
-        | t'' => pred t''
-        end
-    | cond p t e => match eval p with
-        | true => eval t
-        | false => eval e
-        | _ => t
-        end
-    | _ => t
+    | zero => true
+    | succ t' => isnv t'
+    | _ => false
     end.
 
-Compute (eval (cond (iszero (pred zero)) true (succ zero))).
+Fixpoint reduce (t : Term) : option Term :=
+    match t with
+    | cond t t1 _       => Some t1
+    | cond f _ t2       => Some t2
+    | cond k t1 t2      => option_map (fun z => cond z t1 t2) (reduce k)
+    | succ n            => option_map succ (reduce n)
+    | pred zero         => Some zero
+    | pred (succ n)     => if isnv n then Some f else None
+    | pred n            => option_map pred (reduce n)
+    | iszero zero       => Some t
+    | iszero (succ n)   => if isnv n then Some f else None
+    | iszero n          => option_map iszero (reduce n)
+    | _                 => None
+    end.
+
+Fixpoint depth (t : Term) : nat :=
+    match t with
+    | zero | t | f  => 1
+    | succ n        => 1 + depth n
+    | iszero n      => 1 + depth n
+    | pred n        => 1 + depth n
+    | cond p t1 t2  => 1 + (max (depth p) (max (depth t1) (depth t2)))
+    end.
+
+(* too obvious *)
+Lemma le_S : forall (a b : nat), a < b -> S a < S b. Proof. intros. lia. Qed.
+Lemma le_O : forall (a : nat), 0 < S a. Proof. intros. lia. Qed.
+
+(* the measufe might be wrong *)
+Function eval (t : Term) {measure depth t} : Term :=
+    match reduce t with
+    | None      => t
+    | Some t'   => eval t'
+    end.
+Proof.
+    intro tm. induction tm; 
+    intros tm' teq; inversion teq.
+    - destruct (reduce tm) eqn: T.
+      + simpl in H0. inversion H0.
+        simpl. apply le_S.
+        apply IHtm. reflexivity.
+      + inversion H0.
+    - 
+      
+Abort.
