Agda/Arth.agda
@@ -1,0 +1,55 @@
+open import Agda.Builtin.Bool
+open import Agda.Builtin.Maybe
+
+infixl 1 _>>=_
+_>>=_ : {A B : Set} → Maybe A → (A → Maybe B) → Maybe B
+nothing >>= f = nothing
+just a  >>= f = f a
+
+infixl 4 _<$>_
+_<$>_ : {A B : Set} → (A → B) → Maybe A → Maybe B
+f <$> x = x >>= λ i → just (f i)
+
+data Term : Set where
+    true            : Term
+    false           : Term
+    zero            : Term
+    succ            : Term -> Term
+    pred            : Term -> Term
+    iszero          : Term -> Term
+    if_then_else_   : Term -> Term -> Term -> Term
+
+isnv : Term -> Bool
+isnv zero       = true
+isnv (succ n)   = isnv n
+isnv _          = false
+
+reduce : Term -> Maybe Term
+reduce (if true then t1 else _)     = just t1
+reduce (if false then _ else t2)    = just t2
+reduce (if p then t1 else t2)       = do p' <- reduce p
+                                         just (if p' then t1 else t2)
+reduce (pred zero) = just zero
+reduce (pred (succ n)) with (isnv n)
+... | true  = just n
+... | false = nothing
+reduce (pred n) = do n' <- reduce n
+                     just (pred n')
+reduce (succ n) = do n' <- reduce n
+                     just (succ n')
+reduce (iszero zero) = just true
+reduce (iszero (succ n)) with (isnv n)
+... | true  = just false
+... | false = nothing
+reduce (iszero n) = do n' <- reduce n
+                       just (iszero n')
+reduce _ = nothing 
+
+{-# TERMINATING #-}
+eval : Term -> Term
+eval t with (reduce t)
+... | nothing = t
+... | just t' = eval t'
+
+t1 : Term
+t1 = if (if iszero zero then false else true) then succ zero else succ (succ zero)
